@prefix schema: <https://schema.org/>.
@prefix skos: <http://www.w3.org/2004/02/skos/core#>.
@prefix rdf: <http://www.w3.org/1999/02/22-rdf-syntax-ns#>.
@prefix rdfs: <http://www.w3.org/2000/01/rdf-schema#>.
@prefix foaf: <http://xmlns.com/foaf/0.1/>.
@prefix xsd: <http://www.w3.org/2001/XMLSchema#>.
@prefix dcterms: <http://purl.org/dc/terms/>.
@prefix owl: <http://www.w3.org/2002/07/owl#>.
@prefix jsonsc: <https://www.w3.org/2019/wot/json-schema#>.
@prefix jsonsc-ld: <http://w3id.org/jsonsc-ld/>.
@prefix api: <http://purl.org/linked-data/api/vocab>.
@prefix geo: <http://www.w3.org/2003/01/geo/wgs84_pos#>.
@prefix mobivoc: <http://schema.mobivoc.org/#>.
@prefix geosparql: <http://www.opengis.net/ont/geosparql#>.
@prefix gbfs: <https://w3id.org/gbfs#>.

<https://github.com/NABSA/gbfs/blob/v2.2/gbfs.md#free_bike_statusjson> dcterms:description "Describes the vehicles that are available for rent (as of v2.1-RC2).".
dcterms:modified rdf:type rdf:Property.
gbfs:ttl dcterms:description "Number of seconds before the data in the feed will be updated again (0 if the data should always be refreshed).";
    rdf:type rdf:Property;
    rdfs:label "ttl";
    rdfs:domain <https://github.com/NABSA/gbfs/blob/v2.2/gbfs.md#free_bike_statusjson>;
    rdfs:range xsd:integer.
gbfs:version dcterms:description "GBFS version number to which the feed conforms, according to the versioning framework (added in v1.1).";
    rdf:type rdf:Property;
    rdfs:label "version";
    rdfs:domain <https://github.com/NABSA/gbfs/blob/v2.2/gbfs.md#free_bike_statusjson>;
    rdfs:range xsd:string.
gbfs:Bike rdf:type rdfs:Class;
    rdfs:label "Bike".
gbfs:bike_id dcterms:description "Rotating (as of v2.0) identifier of a vehicle.";
    rdf:type rdf:Property;
    rdfs:label "bike_id";
    rdfs:domain gbfs:Bike;
    rdfs:range xsd:string.
geo:lat rdf:type rdf:Property.
geo:long rdf:type rdf:Property.
gbfs:is_reserved dcterms:description "Is the vehicle currently reserved?";
    rdf:type rdf:Property;
    rdfs:label "is_reserved";
    rdfs:domain gbfs:Bike;
    rdfs:range xsd:boolean.
gbfs:is_disabled dcterms:description "Is the vehicle currently disabled (broken)?";
    rdf:type rdf:Property;
    rdfs:label "is_disabled";
    rdfs:domain gbfs:Bike;
    rdfs:range xsd:boolean.
gbfs:rental_uris dcterms:description "Contains rental uris for Android, iOS, and web in the android, ios, and web fields (added in v1.1).";
    rdf:type rdf:Property;
    rdfs:label "rental_uris";
    rdfs:domain gbfs:Bike;
    rdfs:range gbfs:Rental_uris.
gbfs:Rental_uris dcterms:description "Rental uris for Android, iOS, and web.";
    rdf:type rdfs:Class;
    rdfs:label "Rental_uris".
gbfs:android dcterms:description "URI that can be passed to an Android app with an intent (added in v1.1).";
    rdf:type rdf:Property;
    rdfs:label "android";
    rdfs:domain gbfs:Rental_uris;
    rdfs:range xsd:anyURI.
gbfs:ios dcterms:description "URI that can be used on iOS to launch the rental app for this vehicle (added in v1.1).";
    rdf:type rdf:Property;
    rdfs:label "ios";
    rdfs:domain gbfs:Rental_uris;
    rdfs:range xsd:anyURI.
gbfs:web dcterms:description "URL that can be used by a web browser to show more information about renting this vehicle (added in v1.1).";
    rdf:type rdf:Property;
    rdfs:label "web";
    rdfs:domain gbfs:Rental_uris;
    rdfs:range xsd:anyURI.
gbfs:vehicle_type_id dcterms:description "The vehicle_type_id of this vehicle (added in v2.1-RC).";
    rdf:type rdf:Property;
    rdfs:label "vehicle_type_id";
    rdfs:domain gbfs:Bike;
    rdfs:range xsd:string.
gbfs:last_reported dcterms:description "The last time this vehicle reported its status to the operator's backend in POSIX time (added in v2.1-RC).";
    rdf:type rdf:Property;
    rdfs:label "last_reported";
    rdfs:domain gbfs:Bike;
    rdfs:range xsd:decimal.
gbfs:current_range_meters dcterms:description "The furthest distance in meters that the vehicle can travel without recharging or refueling with the vehicle's current charge or fuel (added in v2.1-RC).";
    rdf:type rdf:Property;
    rdfs:label "current_range_meters";
    rdfs:domain gbfs:Bike;
    rdfs:range xsd:decimal.
gbfs:station_id dcterms:description "Identifier referencing the station_id if the vehicle is currently at a station (added in v2.1-RC2).";
    rdf:type rdf:Property;
    rdfs:label "station_id";
    rdfs:domain gbfs:Bike;
    rdfs:range xsd:string.
gbfs:pricing_plan_id dcterms:description "The plan_id of the pricing plan this vehicle is eligible for (added in v2.1-RC2).";
    rdf:type rdf:Property;
    rdfs:label "pricing_plan_id";
    rdfs:domain gbfs:Bike;
    rdfs:range xsd:string.
